pure/GD.thy
@@ -1801,6 +1801,7 @@ apply (induct y, simp)
 apply (unfold_def cpair_def, simp)+
 done
 
+find_theorems name: "cpair"
 
 lemma cpair_suc [auto]: "x N \<Longrightarrow> y N \<Longrightarrow> \<langle>x, S(y)\<rangle> = \<langle>x, y\<rangle> + x + S(y) + 1"
 apply (rule eqSym)
